update for class

theories/type_systems/stlc/closed.v
@@ -1,4 +1,4 @@
-From ffpl.lib Require Import prelude.
+From ffpl.lib Require Import prelude sets.
 From ffpl.type_systems.stlc Require Export lang.
 
 (** Open and closed expressions.
@@ -8,26 +8,26 @@ that says whether a set [X] contains all free variables:
 [is_closed X e] evaluates to [true] iff all free variables in [e] are contained in [X].
 We define this as a functon that returns a [bool], i.e. this actually computes an
 answer that is either [true] or [false]. *)
-Fixpoint is_closed (X : list string) (e : expr) : bool :=
+Fixpoint is_closed (X : gset string) (e : expr) : bool :=
   match e with
   | Var x => bool_decide (x `elem` X)
-  | Lam x e => is_closed (x :: X) e
+  | Lam x e => is_closed ({[x]} `union` X) e
   | LitInt _ => true
   | App e1 e2
   | Plus e1 e2 => is_closed X e1 && is_closed X e2
   end.
 
 (** We can compute with this definition. *)
-Compute (is_closed [] (LitInt 0)).
-Compute (is_closed [] (Var "x")).
-Compute (is_closed ["x"] (Var "x")).
+Compute (is_closed empty (LitInt 0)).
+Compute (is_closed empty (Var "x")).
+Compute (is_closed {["x"]} (Var "x")).
 
 (** [closed X e] is the propositional version of [is_closed X e]:
 [closed X e] has type [Prop], not [bool]. *)
 Notation closed X e := (Is_true (is_closed X e)).
 
 (** Defining it like this means we can do proofs "by computation". *)
-Example lit_is_closed z : closed [] (LitInt z).
+Example lit_is_closed z : closed empty (LitInt z).
 Proof. simpl. done. Qed.
 
 (** We show some key properties of [closed].
@@ -36,40 +36,8 @@ somewhat tricky to work with); we will provide all the results you need. *)
 Lemma closed_weaken X Y e : closed X e -> subseteq X Y -> closed Y e.
 Proof. revert X Y; induction e; naive_solver (eauto; set_solver). Qed.
 
-Lemma closed_weaken_nil X e : closed [] e -> closed X e.
-Proof. intros. by apply closed_weaken with [], list_subseteq_nil. Qed.
-
-Lemma closed_subst X Y e x es :
-  closed Y es -> closed (x :: X) e -> closed (X ++ Y) (subst x es e).
-Proof.
-  (** [induction ... in X |- *] is a short-hand for generalizing X in the
-  induction hypothesis. *)
-  induction e as [y|y e IH|e1 e2|n|e1 e2] in X |- *; simpl; intros Hc1 Hc2; eauto.
-  - eapply bool_decide_unpack, elem_of_cons in Hc2 as [->|Hc2].
-    + destruct decide; try congruence. eapply closed_weaken; eauto with set_solver.
-    + destruct decide.
-      * eapply closed_weaken; eauto with set_solver.
-      * simpl. eapply bool_decide_pack. set_solver.
-  - destruct decide as [Heq|].
-    + eapply closed_weaken; eauto. set_solver.
-    + rewrite app_comm_cons. eapply IH; eauto.
-      eapply closed_weaken; eauto. set_solver.
-  - eapply andb_True. eapply andb_True in Hc2 as [H1 H2].
-    split; eauto.
-  - eapply andb_True. eapply andb_True in Hc2 as [H1 H2].
-    split; eauto.
-Qed.
-
-Lemma closed_subst_nil X e x es :
-  closed [] es -> closed (x :: X) e -> closed X (subst x es e).
-Proof.
-  intros Hc1 Hc2. eapply closed_subst in Hc1; eauto.
-  revert Hc1. rewrite right_id //.
-Qed.
-
-Lemma closed_do_subst' X e x es :
-  closed [] es -> closed (x :: X) e -> closed X (subst x es e).
-Proof. destruct x; eauto using closed_subst_nil. Qed.
+Lemma closed_weaken_nil X e : closed empty e -> closed X e.
+Proof. intros. by apply closed_weaken with empty, empty_subseteq. Qed.
 
 Lemma subst_closed X e x es : closed X e -> ~(x `elem` X) -> subst x es e = e.
 Proof.
@@ -77,5 +45,5 @@ Proof.
     repeat case_decide; simplify_eq; simpl; f_equal; intuition eauto with set_solver.
 Qed.
 
-Lemma subst_closed_nil e x es : closed [] e -> subst x es e = e.
-Proof. intros. apply subst_closed with []; set_solver. Qed.
+Lemma subst_closed_nil e x es : closed empty e -> subst x es e = e.
+Proof. intros. apply subst_closed with empty; done || set_solver. Qed.
