theories/type_systems/stlc/logrel_class.v
@@ -1,0 +1,176 @@
+From stdpp Require Import base relations.
+From ffpl.lib Require Import prelude sets maps.
+From ffpl.type_systems.stlc Require Import lang notation types parallel_subst.
+From Equations Require Import Equations.
+
+Implicit Types
+  (Gamma : typing_context)
+  (v : val)
+  (e : expr)
+  (A : type).
+
+
+(** ** Definition of the logical relation. *)
+
+(** Convince Coq that our logical relation is well-defined. *)
+Equations type_size (t : type) : nat :=
+  type_size Int := 1;
+  type_size (Fun A B) := type_size A + type_size B + 1.
+Equations mut_measure (v : val + expr) (t : type) : nat :=
+  mut_measure (inr e) t := 1 + type_size t;
+  mut_measure (inl v) t := type_size t.
+
+Equations type_interp (v : val + expr) (t : type) : Prop by wf (mut_measure v t) := {
+  type_interp (inl v) Int =>
+    exists z : Z, v = z ;
+  type_interp (inl v) (A -> B) =>
+    exists x e, v = @LamV x e /\ closed empty v /\
+      forall v',
+        type_interp (inl v') A ->
+        type_interp (inr (subst x v' e)) B;
+
+  type_interp (inr e) t =>
+    exists v, big_step e v /\ type_interp (inl v) t
+}.
+Next Obligation.
+  simp mut_measure. simp type_size. lia.
+Qed.
+Next Obligation.
+  simp mut_measure. simp type_size.
+  destruct A; simp mut_measure; simp type_size; lia.
+Qed.
+
+(** We derive the expression/value relation. *)
+Notation sem_val_rel t v := (type_interp (inl v) t).
+Notation sem_expr_rel t e := (type_interp (inr e) t).
+
+(** *** Semantic typing of contexts *)
+Implicit Types
+  (gamma : gmap string expr).
+
+Inductive sem_ctx_rel : typing_context -> (gmap string expr) -> Prop :=
+  | sem_ctx_rel_empty : sem_ctx_rel empty empty
+  | sem_ctx_rel_insert Gamma gamma v x A :
+    sem_val_rel A v ->
+    sem_ctx_rel Gamma gamma ->
+    sem_ctx_rel (<[x := A]> Gamma) (<[x := of_val v]> gamma).
+
+(** The semantic typing judgment *)
+Definition sem_typed Gamma e A :=
+  closed (dom Gamma) e /\
+  forall gamma, sem_ctx_rel Gamma gamma -> sem_expr_rel A (subst_map gamma e).
+Notation "Gamma |= e : A" := (sem_typed Gamma e A) (at level 74, e, A at next level).
+
+(** We start by proving a couple of helper lemmas that will be useful later. *)
+
+Lemma val_rel_closed v A:
+  sem_val_rel A v -> closed empty v.
+Proof.
+  induction A; simp type_interp.
+  - intros [z ->]. done.
+  - intros (x & e & -> & Hcl & _). done.
+Qed.
+
+Lemma ctx_rel_closed Gamma gamma :
+  sem_ctx_rel Gamma gamma -> subst_closed empty gamma.
+Proof.
+  induction 1; rewrite /subst_closed.
+  - intros x e. rewrite lookup_empty. done.
+  - intros y e. rewrite lookup_insert_Some.
+    intros [[-> <-]|[Hne Hlook]].
+    + eapply val_rel_closed. done.
+    + eapply IHsem_ctx_rel; last done.
+Qed.
+
+(** This is basically the inversion lemma for [sem_ctx_rel]:
+if a variable exists in Gamma, then we can find a suitable value in gamma. *)
+Lemma ctx_rel_lookup Gamma gamma x A :
+  sem_ctx_rel Gamma gamma ->
+  Gamma !! x = Some A ->
+  exists v, gamma !! x = Some (of_val v) /\ sem_val_rel A v.
+Proof.
+  induction 1 as [|Gamma gamma v y B Hval Hctx IH].
+  - rewrite lookup_empty. done.
+  - rewrite lookup_insert_Some. intros [[-> ->]|[Hne Hlook]].
+    + exists v. split; first by rewrite lookup_insert_eq.
+      eauto.
+    + eapply IH in Hlook as (w & Hlook & Hval_w).
+      eexists. split; first by rewrite lookup_insert_ne.
+      eauto.
+Qed.
+
+Lemma ctx_rel_dom Gamma gamma :
+  sem_ctx_rel Gamma gamma -> dom Gamma = dom gamma.
+Proof.
+  induction 1; first by rewrite !dom_empty.
+  rewrite !dom_insert. congruence.
+Qed.
+
+(** Lemma 17: Value Inclusion *)
+Lemma val_inclusion A v :
+  sem_val_rel A v -> sem_expr_rel A (of_val v).
+Proof. (* FILL IN HERE *) Admitted.
+
+(** *** Compatibility lemmas *)
+
+(** Lemma 19 *)
+Lemma compat_int Gamma z : Gamma |= (LitInt z) : Int.
+Proof. (* DONE IN CLASS *) Admitted.
+
+(** Lemma 20 *)
+Lemma compat_var Gamma x A :
+  Gamma !! x = Some A ->
+  Gamma |= (Var x) : A.
+Proof. (* DONE IN CLASS *) Admitted.
+
+(** Lemma 21 *)
+Lemma compat_app Gamma e1 e2 A B :
+  Gamma |= e1 : (A -> B) ->
+  Gamma |= e2 : A ->
+  Gamma |= (e1 e2) : B.
+Proof. (* DONE IN CLASS *) Admitted.
+
+(* Compatibility for [lam] unfortunately needs a very technical helper lemma. *)
+Lemma lam_closed Gamma gamma x A e :
+  closed (dom (<[x:=A]> Gamma)) e ->
+  sem_ctx_rel Gamma gamma ->
+  closed ∅ (lam: x, subst_map (delete x gamma) e)%V.
+Proof.
+  intros Hcl Hctxt. simpl. eapply closed_subst_map.
+  - eapply closed_weaken; first done.
+    rewrite dom_delete dom_insert (ctx_rel_dom Gamma gamma) //.
+    intros y. destruct (decide (x = y)); set_solver.
+  - eapply subst_closed_weaken, ctx_rel_closed; last done.
+    + set_solver.
+    + apply map_delete_subseteq.
+Qed.
+
+(** Lemma 22 *)
+Lemma compat_lam Gamma x e A B :
+  (<[ x := A ]> Gamma) |= e : B ->
+  Gamma |= (Lam x e) : (A -> B).
+Proof. (* DONE IN CLASS *) Admitted.
+
+(** Omitted in the lecture notes *)
+Lemma compat_add Gamma e1 e2 :
+  Gamma |= e1 : Int ->
+  Gamma |= e2 : Int ->
+  Gamma |= (e1 + e2) : Int.
+Proof. (* FILL IN HERE *) Admitted.
+
+(** Theorem 23 *)
+Theorem sem_soundness Gamma e A :
+  (Gamma |- e : A)%ty ->
+  Gamma |= e : A.
+Proof. (* FILL IN HERE *) Admitted.
+
+(** Corollary 24 *)
+Corollary termination e A :
+  (empty |- e : A)%ty ->
+  exists v, big_step e v.
+Proof. (* DONE IN CLASS *) Admitted.
+
+(* In-class exercise:
+- [type_safety] in types_class2.v
+  (bonus exercise: complete [type_substitution])
+- [val_inclusion], [compat_add] and [sem_soundness] above. *)
