theories/type_systems/stlc/types_class2.v
@@ -1,51 +1,24 @@
 From stdpp Require Import base relations tactics.
 From ffpl.lib Require Import prelude sets maps.
-From ffpl.type_systems.stlc Require Import lang notation.
+From ffpl.type_systems.stlc Require Import lang closed notation.
 
 (** ** Syntactic typing *)
-(** In the Coq formalization, we exclusively define runtime typing (Curry-style). *)
-(** It will be an exercise to consider Church-style typing. *)
 
 Inductive type : Set :=
   | Int
   | Fun (A B : type).
-
-(** In the lecture, we defined contexts 'Gamma' inductively.
-However, in the end we are just using them as an association map that maps
-variable names to types, so we use a type of finite partial maps in Coq: [gmap K
-V]. Its key operations are:
-- lookup: With [m : gmap K V] and [k : K], the term [m !! k] of type [option V]
-  is a lookup of [k] in [m] that returns [Some v] if [k] maps to [v] and [None]
-  if [k] does not currently map to anything.
-- insert: With [m : gmap K V], [k : K], and [v : V], the term [ <[ k := v ]> m ]
-  is the map where [k] maps to [v] and everything else maps the same way it does
-  in [m]. This can be used to insert a new key into a map and to overwrite an
-  already existing key.
-In our case, variable names are strings, so the type of contexts is defined as
-follows: *)
-Notation typing_context := (gmap string type).
-
-(** This command tells Coq that when a variable is named [Gamma] or [Gamma'] or
-[Gamma1] or something like that, then it should implicitly have type
-[typing_context], and similar for the other names and types. This avoids type
-annotations in the rest of the file. *)
+Definition typing_context := gmap string type.
 Implicit Types
   (Gamma : typing_context)
   (v : val)
   (e : expr)
   (A : type)
   (x : string).
-
-(** We define notation for types in a new scope with delimiter [ty].
-  See below for an example. *)
 Declare Scope FType_scope.
 Delimit Scope FType_scope with ty.
 Bind Scope FType_scope with type.
 Infix "->" := Fun : FType_scope.
 
-(** Typing rules *)
-(** We need to reserve the notation beforehand to already use it when defining the
-   typing rules. *)
 Reserved Notation "Gamma |- e : A" (at level 74, e, A at next level).
 Inductive syn_typed : typing_context -> expr -> type -> Prop :=
   | typed_var Gamma x A :
@@ -67,18 +40,10 @@ Inductive syn_typed : typing_context -> expr -> type -> Prop :=
       Gamma |- e2 : Int ->
       Gamma |- e1 + e2 : Int
 where "Gamma |- e : A" := (syn_typed Gamma e%E A%ty) : FType_scope.
-(** Add constructors to [eauto]'s hint database. *)
 #[export] Hint Constructors syn_typed : core.
 Local Open Scope FType_scope.
-(** Also export the notation (it would otherwise remain local to this file). *)
 Notation "Gamma |- e : A" := (syn_typed Gamma e%E A%ty).
 
-(** a small example *)
-Goal empty |- (lam: "x", 1 + "x")%E : (Int -> Int).
-Proof. eauto. Qed.
-
-(** We derive some inversion lemmas -- this is cleaner than directly
-using the [inversion] tactic everywhere.*)
 Lemma var_inversion Gamma (x : string) A :
   Gamma |- x : A -> Gamma !! x = Some A.
 Proof. inversion 1; subst; auto. Qed.
@@ -86,9 +51,6 @@ Proof. inversion 1; subst; auto. Qed.
 Lemma lam_inversion Gamma (x : string) e C :
   (Gamma |- (lam: x, e) : C) ->
   exists A B, C = (A -> B)%ty /\ <[x:=A]> Gamma |- e : B.
-(** [eauto] has a "fuel" parameter that tells it how long it shoud keep
-going before giving up on a goal. Here we need to increase the fuel to 10
-to enable it to solve all goals. *)
 Proof. inversion 1; subst; eauto 10. Qed.
 
 Lemma lit_int_inversion Gamma (n : Z) A : (Gamma |- n : A) -> A = Int.
@@ -105,13 +67,11 @@ Lemma plus_inversion Gamma e1 e2 B :
 Proof. inversion 1; subst; eauto. Qed.
 
 (** * Progress *)
-
-(** Canonical forms lemmas (Lemma 7) *)
 Lemma canonical_values_arr Gamma e A B :
   Gamma |- e : (A -> B) ->
   is_val e ->
   exists x e', e = (lam: x, e')%E.
-(* CLASS *) Proof.
+Proof.
   inversion 1; simpl; by eauto.
 Qed.
 
@@ -119,18 +79,16 @@ Lemma canonical_values_int Gamma e :
   Gamma |- e : Int ->
   is_val e ->
   exists n: Z, e = n.
-(* CLASS *) Proof.
+Proof.
   inversion 1; simpl; by eauto.
 Qed.
 
-(** Definition 6 *)
 Definition progressive (e : expr) :=
   is_val e \/ exists e', contextual_step e e'.
 
-(** Theorem 8 *)
 Theorem type_progress e A :
   empty |- e : A -> progressive e.
-(* CLASS *) Proof.
+Proof.
   remember empty as Gamma. induction 1 as [??? Hx| | | Gamma e1 e2 A B Hty IH1 _ IH2 | Gamma e1 e2 Hty1 IH1 Hty2 IH2].
   - subst.
     (** The lemma [lookup_empty] shows that [empty !! x = None], which in this
@@ -160,18 +118,12 @@ Qed.
 
 (** * Preservation *)
 
-(** Helper lemmas for base preservation *)
-
-(** We are using various lemmas about maps here, such as [lookup_weaken]
-and [insert_mono]. Use [About] to learn about their statements. *)
-
-(** Lemma 9 *)
 Lemma type_weakening Gamma Delta e A :
   Gamma |- e : A ->
   Gamma `subseteq` Delta ->
   Delta |- e : A.
 Proof.
-  induction 1 in Delta; intros Hsub.
+  induction 1 in Delta |- *; intros Hsub.
   - eauto using lookup_weaken.
   - eauto using insert_mono.
   - eauto.
@@ -179,99 +131,50 @@ Proof.
   - eauto.
 Qed.
 
-(** Lemma 10 *)
 Lemma type_substitution e e' Gamma x A B :
   empty |- e' : A ->
   <[x := A]> Gamma |- e : B ->
   Gamma |- subst x e' e : B.
-(* CLASS *) Proof.
-  intros He'. revert B Gamma; induction e as [y | y | | |]; intros B Gamma; simpl.
-  - intros Hp%var_inversion.
-    (** We could say [destruct (decide (x = y))] here to make progress in the proof,
-    but [destruct] is smart and we can give it a partial term that it will then
-    find in the goal to figure out what we want to do case distinction on. *)
-    destruct (decide _); subst; eauto.
-    + Search (<[?x:=_]> _ !! ?x = Some _).
-      rewrite lookup_insert_eq in Hp. simplify_eq.
-      eapply type_weakening; first done. apply map_empty_subseteq.
-    + rewrite lookup_insert_ne in Hp; last done. auto.
-  - intros (C & D & -> & Hty)%lam_inversion.
-    econstructor. destruct (decide _) as [|Heq]; simplify_eq.
-    + by rewrite insert_insert in Hty.
-    + rewrite insert_commute in Hty; by eauto.
-  - intros (C & Hty1 & Hty2)%app_inversion; eauto.
-  - intros ->%lit_int_inversion. eauto.
-  - intros (-> & Hty1 & Hty2)%plus_inversion; eauto.
-Qed.
+Proof. (* var, app case DONE IN CLASS *) Admitted.
 
-(** Base preservation (Lemma 11) *)
 Lemma type_preservation_base_step e e' A :
   empty |- e : A ->
   base_step e e' ->
   empty |- e' : A.
-(* CLASS *) Proof.
-  intros Hty Hstep. destruct Hstep as [| e1 e2 n1 n2 n3 Heq1 Heq2 Heval]; subst.
-  - eapply app_inversion in Hty as (B & Hty1 & Hty2).
-    eapply lam_inversion in Hty1 as (B' & A' & Heq1 & Hty).
-    simplify_eq. eapply type_substitution; eauto.
-  - eapply plus_inversion in Hty as (-> & Hty1 & Hty2).
-    econstructor.
-Qed.
+Proof. (* DONE IN CLASS *) Admitted.
 
-(** Contextual typing for evaluation context items and evaluation contexts  *)
 Definition ectx_item_typing (Ki : ectx_item) (A B : type) :=
   forall e, empty |- e : A -> empty |- (fill_item Ki e) : B.
-
 Lemma fill_item_typing_decompose Ki e A :
   empty |- fill_item Ki e : A ->
   exists B, empty |- e : B /\ ectx_item_typing Ki B A.
-(* CLASS *) Proof.
-  unfold ectx_item_typing; destruct Ki; simpl; inversion 1; subst; eauto.
-Qed.
+Proof. (* DONE IN CLASS *) Admitted.
 
 Definition ectx_typing (K : ectx) (A B : type) :=
   forall e, empty |- e : A -> empty |- (fill K e) : B.
-
-(** Lemma 12 *)
 Lemma fill_typing_decompose K e A :
   empty |- fill K e : A ->
   exists B, empty |- e : B /\ ectx_typing K B A.
-(* CLASS *) Proof.
-  (** The [in e |- *] here performs automatic generalization over [e]. *)
-  (** Contrary to the proof in the notes, we don't need to generalize [A] here,
-  because prepending a context item to a context list corresponds to
-  precomposing with the context item. *)
+Proof.
   unfold ectx_typing. induction K as [|k K] in e |- *; simpl; eauto.
   intros [B [Hit Hty]]%IHK.
   eapply fill_item_typing_decompose in Hit as [B' [? ?]]; eauto.
 Qed.
 
-(** Lemma 13 *)
 Lemma fill_typing_compose K e A B :
   empty |- e : B ->
   ectx_typing K B A ->
   empty |- fill K e : A.
-(* CLASS *) Proof.
-  intros H1 H2; by eapply H2.
-Qed.
+Proof. (* DONE IN CLASS *) Admitted.
 
-(** Preservation (Theorem 14) *)
 Theorem type_preservation e e' A :
   empty |- e : A ->
   contextual_step e e' ->
   empty |- e' : A.
-(* CLASS *) Proof.
-  intros Hty Hstep. destruct Hstep as [K e1 e2 -> -> Hstep].
-  eapply fill_typing_decompose in Hty as [B [H1 H2]].
-  eapply fill_typing_compose; last done.
-  by eapply type_preservation_base_step.
-Qed.
+Proof. (* DONE IN CLASS *) Admitted.
 
-(** Corollary 15 *)
 Corollary type_safety e1 e2 A:
   empty |- e1 : A ->
   rtc contextual_step e1 e2 ->
   progressive e2.
-(* REMOVE *) Proof.
-  induction 2; eauto using type_progress, type_preservation.
-Qed.
+Proof. (* FILL IN HERE *) Admitted.
